Foundation/Modal/Kripke/Logic/S4Point4.lean
@@ -39,8 +39,8 @@ open Kripke
 
 lemma S4Point4.Kripke.preorder_sobocinski : Logic.S4Point4 = FrameClass.preorder_sobocinski.logic := eq_hilbert_logic_frameClass_logic
 
-instance : ProperSublogic Logic.S4Point3 Logic.S4Point4 := ⟨
-  by
+@[simp]
+theorem S4Point4.proper_extension_of_S4Point4 : Logic.S4Point3 ⊂ Logic.S4Point4 := by
   constructor;
   . rw [S4Point3.Kripke.connected_preorder, S4Point4.Kripke.preorder_sobocinski];
     rintro φ hφ F ⟨_, _⟩;
@@ -66,7 +66,6 @@ instance : ProperSublogic Logic.S4Point3 Logic.S4Point4 := ⟨
           simpa [Semantics.Realize, Satisfies, M];
         use 2;
         omega;
-⟩
 
 end Logic
 
